Core/interlude.v
@@ -1,0 +1,29 @@
+From Coq Require Import ssreflect ssrbool ssrfun Eqdep.
+From mathcomp Require Import ssrnat seq eqtype.
+From fcsl Require Import axioms.
+From fcsl Require Import options.
+
+Lemma has_takedrop {A : Type} (p : pred A) (s : seq A) x :
+        has p s ->
+          s = take (find p s) s ++ [::nth x s (find p s)] ++ drop (find p s).+1 s.
+Proof.
+move=>H.
+set i := find p s.
+have L1 : i < size s by rewrite /i -has_find.
+rewrite -{1}(cat_take_drop i s).
+by rewrite (drop_nth x).
+Qed.
+
+Lemma mem_split {T : eqType} (x : T) (s : seq T) :
+        x \in s -> exists s1, exists s2, s = s1 ++ [:: x] ++ s2.
+Proof.
+move=>H.
+have L : has (pred1 x) s.
+- by case: hasP=>//; elim; exists x=>/=.
+move: (has_takedrop x L).
+set i := find (pred1 x) s.
+rewrite (_ : nth x s i = x); last first.
+- suff : pred1 x (nth x s i) by move/eqP.
+  by apply: nth_find.
+eauto.
+Qed.
