Examples/hashtab.v
@@ -1,0 +1,177 @@
+From mathcomp Require Import ssreflect ssrbool ssrnat eqtype ssrfun seq fintype tuple finfun finset.
+From fcsl Require Import axioms prelude pred ordtype finmap.
+From fcsl Require Import pcm unionmap heap.
+From HTT Require Import domain stmod stsep stlog stlogR.
+From HTT Require Import array kvmaps.
+Set Implicit Arguments.
+Unset Strict Implicit.
+Unset Printing Implicit Defensive.
+Obligation Tactic := auto.
+
+Module HashTab.
+Section HashTab.
+Import FinIter.
+Variables (K : ordType) (V : Type) (buckets : KVmap.Sig K V)
+          (n : nat) (hash : K -> 'I_n).
+Definition hashtab := {array 'I_n -> KVmap.tp buckets}.
+Notation KVshape := (@KVmap.shape _ _ buckets).
+Notation table := (table KVshape).
+
+Definition shape x s :=
+  [Pred h | exists tab bucket,
+           [/\ forall k, fnd k s = fnd k (bucket (hash k)),
+               forall i k, k \in supp (bucket i) -> hash k = i &
+               h \In Array.shape x tab # sepit setT (table tab bucket)] ].
+
+Definition new_loopinv x := forall k,
+  STsep (fun h => k <= n /\ exists tab, h \In Array.shape x tab #
+                   sepit [set x:'I_n | x < k] (table tab (fun x:'I_n => nil K V)),
+         [vfun y => shape y (nil K V)]).
+
+Program Definition new : STsep (emp, [vfun y => shape y (nil K V)]) :=
+  Do (t <-- Array.new _ (KVmap.default buckets);
+      Fix (fun (loop : new_loopinv t) k =>
+           Do (match decP (b := k < n) idP with
+               | left pf => b <-- KVmap.new buckets;
+                            Array.write t (Ordinal pf) b;;
+                            loop k.+1
+               | _ => ret t end)) 0).
+Next Obligation.
+move=>/= arr loop k h /= [Eleq][tab][h1][h2][-> [H1 H2]]; case: decP; last first.
+- move/negP=>Ho; rewrite leq_eqVlt (negbTE Ho) orbF in Eleq.
+  step=>Vh [_ [tab2 H12]].
+  exists tab, (fun _:'I_n => nil K V); split=>//; exists h1, h2; do!split=>//.
+  apply: (tableP2 _ _ _ H2)=>// x; move/eqP: Eleq=>->.
+  by rewrite !in_set ltn_ord.
+move=>Ho; rewrite -[h1 \+ h2]unitL.
+apply: bnd_seq; move=>/= Vs; split; first by exists Unit, (h1 \+ h2).
+move=>y m Hm; case: (Hm Unit (h1 \+ h2))=>// m1 [-> [Vm1]] /[swap] _ {Hm}.
+case: y=>/= b Hm; last by move=>_ _; apply: Hm.
+apply: bnd_seq; move=>/= _; split.
+- exists h1, (m1 \+ h2); do!split=>//; first by rewrite joinCA.
+  by exists tab.
+move=>y m0 Hm0; case: (Hm0 h1 (m1 \+ h2))=>//.
+- by rewrite joinCA.
+- by exists tab.
+move=>m2 [->][Vm2] /[swap] _; move: Hm0.
+case: y=>/=; last by move=>_ _ Hx _ _; apply: (Hx tab).
+move=>[] _ /(_ tab); case=>// E2 V2.
+apply/val_doR=>// _; split=>//.
+exists [ffun z => if z == Ordinal Ho then b else tab z].
+exists m2, (m1 \+ h2); do!split=>//.
+rewrite (sepitS (Ordinal Ho)) in_set leqnn {1}/table ffunE eq_refl.
+exists m1, h2; do!split=>//; first by apply: Hm.
+apply: tableP2 H2=>//.
+- by case=>x ?; rewrite !in_set -val_eqE /= ltnS (leq_eqVlt x); case: ltngtP.
+by move=>x _; rewrite in_set ffunE; case: eqP=>//->; rewrite ltnn.
+Qed.
+Next Obligation.
+move=>/= ? ->; apply: bnd_seq=>/= _ /=; split.
+- by rewrite -[Unit]unitL; exists Unit, Unit.
+move=>y m H Vm; case: y H=>/=; last first.
+- move=>_ H _ _; case: (H Unit Unit)=>//; first by rewrite unitR.
+  by move=>x [_ [_]]; apply.
+move=>arr H; apply: val_do0=>// _; split=>//.
+exists [ffun _ => KVmap.default buckets].
+exists m, Unit; do!split=>//=.
+- by rewrite unitR.
+- case: (H Unit Unit)=>//; first by rewrite unitR.
+  by move=>x [E [_ {}H]]; case: H=>//; rewrite E unitR.
+by rewrite (eq_sepit (s2 := set0)) // sepit0.
+Qed.
+
+(*
+Definition free_loopinv x := forall k,
+  STsep unit (fun h => k <= n /\ exists t, exists b, h \In Array.shape x t #
+                       sepit [set x:'I_n | x >= k] (table t b),
+              fun y i m => y = Val tt /\ m = empty).
+
+Program Definition free x : STsep unit (fun i => exists s, i \In shape x s,
+                                        fun y i m => y = Val tt /\ m = empty) :=
+  Do (Fix (fun (loop : free_loopinv x) k =>
+             Do (Match_dec (dec (k < n))
+                  (fun pf => b <-- Array.read x (Ordinal pf);
+                             KVmap.free b;;
+                             loop k.+1)
+                  (fun _ => Array.free x))) 0).
+Next Obligation.
+move: i H0 H1 H2=>h t b [h1][h2][->][H1][]; case: dec=>[{H} pf H2|]; last first.
+- case: ltnP H (eqn_leq k n)=>// _ -> /=; move/eqP=>-> _.
+  rewrite (eq_sepit set0) ?sepit0; last by case=>y p; rewrite in_set inE leqNgt p.
+  move=>->; rewrite unh0=>D; apply: cons0=>/=; eauto.
+apply: bnd_gh (H1)=>[b' _ [[->]] <-|??[]] //; rewrite pf.
+move: H2; rewrite (sepitS (Ordinal pf)) in_set leqnn /table.
+move=>[h3][h4][->][H2][H3] _; rewrite unCA.
+apply: bnd_do=>[|[]_[_]->|??[]] //=; first by eauto.
+rewrite un0h=>D; apply: cons0=>//; split=>//; exists t; exists b; hauto D.
+apply: tableP2 H3=>//; move=>[y qf]; rewrite !in_set -val_eqE /=.
+by case: eqP=>[->|]; rewrite ?ltnn // leq_eqVlt; case: ltngtP=>// ->.
+Qed.
+Next Obligation.
+by apply: cons0=>//=; [case: H0=>t [b][_][_]; eauto| apply: shapeD H0].
+Qed.
+
+Program
+Definition insert x k v : STsep unit (fun i => exists s, i \In shape x s,
+                                      fun y i m => forall s, i \In shape x s ->
+                                        m \In shape x (ins k v s) /\ y = Val tt) :=
+  Do (b <-- Array.read x (hash k);
+      KVmap.insert b k v).
+Next Obligation.
+apply: (ghost H) H0=>s [t][b][H1][H2][h1][h2][->][H3][H4].
+apply: bnd_gh (H3)=>[b' _ [[->]] <-|??[]] //; move: H4.
+rewrite (sepitT1 (hash k)) /table=>[[h2']][h3][->][H4][H5] _; rewrite unCA.
+apply: val_gh H4=>[[] h2'' [H4'] _ D|??[]] //; split=>//.
+set b'' := [eta b with (hash k) |-> ins k v (b (hash k))].
+exists t; exists (b'' : 'I_n -> {fmap K -> V}); do !split.
+- move=>k'; rewrite /b'' /= fnd_ins.
+  case: ifP=>T1; first by rewrite (eqP T1) eq_refl fnd_ins eq_refl.
+  case: ifP=>T2 //; first by rewrite fnd_ins T1 -(eqP T2).
+- move=>i' k'; rewrite /b'' /=; case: eqP=>[->|_]; last by apply: H2.
+  by rewrite supp_ins inE /=; case: eqP=>[->|_] //=; last by apply: H2.
+rewrite (sepitT1 (hash k)) unCA {1}/table /= eq_refl in D * => D; hauto D.
+by apply: tableP H5=>// y; rewrite !in_set andbT /b'' /=; move/negbTE=>->.
+Qed.
+
+Program
+Definition remove x k : STsep unit (fun i => exists s, i \In shape x s,
+                                    fun y i m => forall s, i \In shape x s ->
+                                      m \In shape x (rem k s) /\ y = Val tt) :=
+  Do (b <-- Array.read x (hash k);
+      KVmap.remove b k).
+Next Obligation.
+apply: (ghost H) H0=>s [t][b][H1][H2][h1][h2][->][H3][H4].
+apply: bnd_gh (H3)=>[b' _ [[->]] <-|??[]] //; move: H4.
+rewrite (sepitT1 (hash k)) /table=>[[h2']][h3][->][H4][H5] _; rewrite unCA.
+apply: val_gh H4=>[[] h2'' [H4'] _ D|??[]] //; split=>//.
+set b'' := [eta b with (hash k) |-> rem k (b (hash k))].
+exists t; exists (b'' : 'I_n -> fmap K V); do !split.
+- move=>k'; rewrite /b'' /= fnd_rem.
+  case: ifP=>T1; first by rewrite (eqP T1) eq_refl fnd_rem eq_refl.
+  case: ifP=>T2 //; first by rewrite fnd_rem T1 -(eqP T2).
+- move=>i' k'; rewrite /b'' /=; case: eqP=>[->|_]; last by apply: H2.
+  by rewrite supp_rem inE /=; case: eqP=>[->|_] //=; last by apply: H2.
+rewrite (sepitT1 (hash k)) unCA {1}/table /= eq_refl in D * => D; hauto D.
+by apply: tableP H5=>// y; rewrite !in_set andbT /b'' /=; move/negbTE=>->.
+Qed.
+
+Program Definition lookup x k :
+  STsep (option V) (fun i => exists s, i \In shape x s,
+                    fun y i m => forall s, i \In shape x s ->
+                                   m \In shape x s /\ y = Val (fnd k s)) :=
+  Do (b <-- Array.read x (hash k);
+      KVmap.lookup b k).
+Next Obligation.
+apply: (ghost H) H0=>s [t][b][H1][H2][h1][h2][->][H3][H4].
+apply: bnd_gh (H3)=>[b' _ [[->]] <-|??[]] //; move: H4.
+rewrite (sepitT1 (hash k)) /table=>[[h2']][h3][->][H4][H5] _; rewrite unCA.
+apply: val_gh H4=>[a h2'' [H4'] [->] {D} D|??[]] //; eauto; rewrite H1; split=>//.
+exists t; exists b; do !split=>//.
+by rewrite (sepitT1 (hash k)) unCA in D * => D; hauto D.
+Qed.
+
+Definition HashTab := KVmap.make (Array null) shapeD shape_invert new free insert remove lookup.
+*)
+End HashTab. End HashTab.
+
+(*Definition HT K V := HashTab.HashTab (AssocList.AssocList K V).*)
